verified/entry.i.dfy
@@ -1,0 +1,109 @@
+include "kev_common.s.dfy"
+include "ARMdef.dfy"
+include "pagedb.s.dfy"
+include "smcapi.s.dfy"
+
+//-----------------------------------------------------------------------------
+// Untrusted Functional Model of Addrspace Entry
+//-----------------------------------------------------------------------------
+// This model is untrusted. Its security is verified by proofs in entry.s.dfy.
+// By proving that the spartan implementation produces the same final state as
+// these pure functions, the spartan implementation is ensured to have the
+// same properties.
+
+function enterDispatchFunctional(stateIn:state, dispPage: PageNr, arg1: int, arg2: int,
+    arg3: int, pageDbIn:PageDb) : state
+    requires ValidState(stateIn);
+	requires validPageDb(pageDbIn);
+    //TODO requires pageDb corresponds to stateIn
+    // This does not have a PageDbOut because it does not change the PageDb
+    // May need lemma to ensure s' corresponds to pageDbIn still
+{
+	reveal_validPageDb();
+	var p_out := smc_enter(pageDbIn, dispPage, arg1, arg2, arg3);
+	var pageDbOut := p_out.0;
+	var errOut := p_out.1;
+	if(errOut != KEV_ERR_SUCCESS()) then
+		// Note: can possibly avoid overspecifying by only requiring the assembly to match the 
+		// result of this function whenever there is no error, and just requiring that
+        // stateOut corresponds to PageDbIn in either case
+		stateIn
+	else
+		reveal_ValidRegState();
+		var addrspacePage := pageDbIn[dispPage].addrspace;
+		var addrspace := pageDbIn[addrspacePage].entry;
+
+		var confOut := stateIn.conf.(m := User, ns := Secure, l1p := addrspace.l1ptnr);
+		var regsOut := stateIn.regs[R0 := arg1][R1 := arg2][R2 := arg3];
+	
+        // This won't be necessary to prove the safety property.
+		var sp_usr := stateIn.regs[SP(User)];
+		var lr_usr := stateIn.regs[LR(User)];
+		var lr_svc := stateIn.regs[LR(Supervisor)];
+		var lr_abt := stateIn.regs[LR(Abort)];
+		var lr_und := stateIn.regs[LR(Undefined)];
+		var globsOut := stateIn.m.globals[OSymbol("sp_usr") := [sp_usr]]
+			    [OSymbol("lr_usr") := [lr_usr]][OSymbol("lr_svc") := [lr_svc]]
+			    [OSymbol("lr_abt") := [lr_abt]][OSymbol("lr_und") := [lr_und]];		
+		
+        var mOut := stateIn.m.(globals := globsOut);
+        
+        // TODO? set FIQ, IRQ bits so interrupts are taken to monitor mode
+            // Only needed with more detailed interrupt model in ARMdef
+		
+        State(regsOut, mOut, confOut)
+}
+
+function enterReturnFunctional(stateIn:state) : state
+{
+    //TODO 
+    stateIn
+}
+
+function svc(stateIn:state) : state
+{
+    var s' := stateIn;
+    // TODO
+    enterReturnFunctional(s')
+}
+
+function irq(stateIn:state) : state
+{
+    // TODO
+    var s' := stateIn;
+    enterReturnFunctional(s')
+}
+
+function fiq(stateIn:state) : state
+{
+    // TODO
+    var s' := stateIn;
+    enterReturnFunctional(s')
+}
+
+function abort(stateIn:state) : state
+{
+    // TODO
+    var s' := stateIn;
+    enterReturnFunctional(s')
+}
+
+// svc
+    // change to monitor mode + disable interrupts (cpsid)
+        // Need interrupt model for this to matter
+    // return success + return value of call
+
+// irq / fiq
+    // mark pending irq/fiq
+    // check spsr for mode
+        // if not -> we were in another handler, go handle it.
+        // (need more detailed model of exceptions for this to matter)
+    // save context in dispatcher
+
+// dispatch_return
+    // restore spsr
+    // restore non-volatiles
+
+// leave secure world
+    // set NS bit
+    // Clear FIQ/IRQ bits so interrupts stay in normal
