verified/entry.s.dfy
@@ -1,0 +1,142 @@
+include "kev_common.s.dfy"
+include "ARMdef.dfy"
+include "pagedb.s.dfy"
+include "pagedb.i.dfy"
+include "smcapi.s.dfy"
+include "smcfunctional.i.dfy"
+
+predicate entryState(s:state, d:PageDb)
+{
+    reveal_validPageDb();
+    ValidState(s) && SaneMem(s.m) && validPageDb(d) &&
+    (validPageDbImpliesClosedRefs(d); pageDbCorresponds(s.m, d)) &&
+    validL1PTPage(d, s.conf.l1p) && !stoppedAddrspace(d, s.conf.l1p)
+}
+
+// All memory addresses except the ones in the active l1 page table
+// have their contents preserved
+predicate MemInvariantExceptAddrspace(s:state, s':state, d:PageDb)
+    requires entryState(s, d)
+{
+    ValidState(s') && AlwaysInvariant(s, s') &&
+    forall i :: i in s.m.addresses && !memInAddrspace(d, s.conf.l1p, i) ==>
+        s.m.addresses[i] == s'.m.addresses[i]
+}
+
+predicate pageInAddrspace(d:PageDb, l1p:PageNr, p:PageNr)
+	requires validPageNr(p) && validL1PTPage(d, l1p)
+    requires (validPageDbImpliesWellFormed(d); !stoppedAddrspace(d, l1p))
+{
+    reveal_validPageDb();
+    !stoppedAddrspace(d, l1p) && 
+    var l1pt := d[l1p].entry.l1pt;
+    l1p == p || Just(p) in l1pt ||
+    exists p' :: Just(p') in l1pt && pageInL2PT(d[p'].entry.l2pt,p)
+}
+
+predicate memInAddrspace(d:PageDb, l1p:PageNr, m: mem)
+    requires validL1PTPage(d, l1p)
+    requires (validPageDbImpliesWellFormed(d); !stoppedAddrspace(d, l1p))
+{
+    exists p :: validPageNr(p) && pageInAddrspace(d, l1p, p) && addrInPage(m, p)
+}
+
+predicate pageInL2PT(l2pt:seq<L2PTE>, p:PageNr)
+{
+    exists l2pte :: l2pte in l2pt && (match l2pte
+        case NoMapping => false
+        case SecureMapping(p', w, e) => w && p' == p
+        case InsecureMapping(p') => p' == p)
+}
+
+//-----------------------------------------------------------------------------
+// Assumptions about user mode execution of the addrspace
+//-----------------------------------------------------------------------------
+function {:axiom} addrspaceHavoc(s:state, d:PageDb) : state
+    requires entryState(s, d)
+    ensures var s' := addrspaceHavoc(s, d);
+        MemInvariantExceptAddrspace(s, s', d) && SaneMem(s'.m) &&
+        s'.conf == s.conf
+
+function {:axiom} addrspaceReturn(s:state, d:PageDb) : state
+    requires entryState(s, d)
+    ensures 
+        addrspaceReturn(s, d) == svc(s)   ||
+        addrspaceReturn(s, d) == irq(s)   ||
+        addrspaceReturn(s, d) == fiq(s)   ||
+        addrspaceReturn(s, d) == abort(s)
+
+
+//-----------------------------------------------------------------------------
+// Addrspace entry / return path
+//-----------------------------------------------------------------------------
+
+function entry(s:state, disp: PageNr, a1: int, a2: int, a3: int, d:PageDb) : state
+    requires entryState(s, d)
+    // TODO requires pageDbCorresponds
+{
+    var s1 := enterDispatchFunctional(s, disp, a1, a2, a3, d);
+    assume false; // TODO need premium enterDispatchFunctional
+    var s2 := addrspaceHavoc(s1, d);
+    var s3 := addrspaceReturn(s2, d);
+    s3
+}
+
+//-----------------------------------------------------------------------------
+// Safety poperties of the monitor/addrspace boundary
+//-----------------------------------------------------------------------------
+
+// The pages owned by other addrspaces are preserved
+predicate {:opaque} addrspaceContentsPreservedExcept(s:state, s':state, disp:PageNr, d: PageDb)
+    requires entryState(s, d)
+    requires validDispatcherPage(d, disp)
+{
+    reveal_validPageDb();
+    var a := d[disp].addrspace;
+    ValidState(s') && AlwaysInvariant(s, s') &&
+    forall a' :: validAddrspacePage(d, a') && a' != a && !stoppedAddrspace(d, a') ==>
+        (var l1' := d[a'].entry.l1ptnr;
+        forall m :: memInAddrspace(d, l1', m) ==>
+            s.m.addresses[m] == s'.m.addresses[m])
+}
+
+// // Probaby needed to prove next lemma
+// lemma addrspaceHavocPreservesPageDb(s:state, d:PageDb)
+//     requires entryState(s, d)
+//     ensures var s' := addrspaceHavoc(s, d);
+//         (validPageDbImpliesClosedRefs(d); pageDbCorresponds(s'.m, d))
+// {
+//     //TODO PROVEME
+// 	assume false;
+// }
+// 
+// lemma addrspaceExecutePreservesPageDb(s:state, d:PageDb)
+//     requires entryState(s, d)
+//     ensures var s' := addrspaceExecute(s, d, a);
+//         (validPageDbImpliesClosedRefs(d); pageDbCorresponds(s'.m, d))
+// {
+//     //TODO PROVEME
+// 	assume false;
+// }
+
+
+lemma entryPreservesOtherAddrspaces(s:state, disp:PageNr, a1:int, a2:int, a3:int, d:PageDb)
+    requires entryState(s, d)
+    ensures  validDispatcherPage(d, disp)
+    ensures  var s' := entry(s, disp, a1, a2, a3, d);
+        addrspaceContentsPreservedExcept(s, s', disp, d)
+{
+    //TODO prove 
+    assume false;
+}
+
+
+//-----------------------------------------------------------------------------
+// Liveness Properties of the monitor/addrspace bondary
+//-----------------------------------------------------------------------------
+
+// args of smc_enter reach r0-r3 ?
+
+// The sequence enter -> execute -> return -> enter -> execute restores the
+    // context from the first execute?
+
